wip: specialized bignum

code/k256/Hacl.K256.Field.fst
@@ -6,6 +6,7 @@ open FStar.Mul
 
 open Lib.IntTypes
 open Lib.Buffer
+open Lib.ByteBuffer
 
 module ST = FStar.HyperStack.ST
 module LSeq = Lib.Sequence
@@ -13,277 +14,181 @@ module BSeq = Lib.ByteSequence
 
 module S = Spec.K256
 
-module BD = Hacl.Bignum.Definitions
-module BN = Hacl.Bignum
-module BR = Hacl.Bignum.ModReduction
-module AM = Hacl.Bignum.AlmostMontgomery
-module BB = Hacl.Bignum.Base
-
-module SN = Hacl.Spec.Bignum
-module SD = Hacl.Spec.Bignum.Definitions
+module BI = Hacl.Spec.K256.Field52
+module BL = Hacl.Spec.K256.Field52.Lemmas
+module BDL = Hacl.Spec.K256.Field52.Definitions.Lemmas
 
 #set-options "--z3rlimit 50 --fuel 0 --ifuel 0"
 
-(**
-  This is a naive implementation of field arithmetic for testing purposes
-*)
+let make_u64_4 out (f0,f1,f2,f3) =
+  out.(0ul) <- f3;
+  out.(1ul) <- f2;
+  out.(2ul) <- f1;
+  out.(3ul) <- f0
 
-let make_u64_4 out (f0, f1, f2, f3) =
+
+let make_u52_5 out (f0,f1,f2,f3,f4) =
   out.(0ul) <- f0;
   out.(1ul) <- f1;
   out.(2ul) <- f2;
   out.(3ul) <- f3;
-  let h = ST.get () in
-  SD.bn_eval_unfold_i (as_seq h out) 4;
-  SD.bn_eval_unfold_i (as_seq h out) 3;
-  SD.bn_eval_unfold_i (as_seq h out) 2;
-  SD.bn_eval_unfold_i (as_seq h out) 1;
-  SD.bn_eval0 (as_seq h out)
+  out.(4ul) <- f4
 
 
 let make_prime_k256 () =
   [@inline_let]
   let r =
-   (u64 0xfffffffefffffc2f,
-    u64 0xffffffffffffffff,
-    u64 0xffffffffffffffff,
-    u64 0xffffffffffffffff) in
+   (u64 0xffffefffffc2f,
+    u64 0xfffffffffffff,
+    u64 0xfffffffffffff,
+    u64 0xfffffffffffff,
+    u64 0xffffffffffff) in
 
-  assert_norm (as_nat4 r = S.prime);
+  assert_norm (as_nat5 r = S.prime);
+  assert_norm (0xffffffffffff <= max48);
+  assert_norm (0xfffffffffffff <= max52);
   r
 
 
 let make_order_k256 () =
   [@inline_let]
   let r =
-   (u64 0xbfd25e8cd0364141,
-    u64 0xbaaedce6af48a03b,
-    u64 0xfffffffffffffffe,
-    u64 0xffffffffffffffff) in
+   (u64 0x25e8cd0364141,
+    u64 0xe6af48a03bbfd,
+    u64 0xffffffebaaedc,
+    u64 0xfffffffffffff,
+    u64 0xffffffffffff) in
 
-  assert_norm (as_nat4 r = S.q);
+  assert_norm (as_nat5 r = S.q);
+  assert_norm (0xffffffffffff <= max48);
+  assert_norm (0xfffffffffffff <= max52);
   r
 
 
 let make_b_k256 () =
   [@inline_let]
-  let r = (u64 0x7, u64 0, u64 0, u64 0) in
-  assert_norm (as_nat4 r = S.b);
+  let r = (u64 0x7, u64 0, u64 0, u64 0, u64 0) in
+  assert_norm (as_nat5 r = S.b);
   r
 
 
 [@CInline]
 let is_felem_zero_vartime f =
   let h0 = ST.get () in
-  let m = BN.bn_is_zero_mask nlimb f in
-  SN.bn_is_zero_mask_lemma (as_seq h0 f);
-  BB.unsafe_bool_of_limb m
+  BL.is_felem_zero_vartime5_lemma (as_felem5 h0 f);
+  BI.is_felem_zero_vartime5 (f.(0ul), f.(1ul), f.(2ul), f.(3ul), f.(4ul))
 
 
 [@CInline]
 let is_felem_eq_vartime f1 f2 =
   let h0 = ST.get () in
-  let m = BN.bn_eq_mask nlimb f1 f2 in
-  SN.bn_eq_mask_lemma (as_seq h0 f1) (as_seq h0 f2);
-  BB.unsafe_bool_of_limb m
-
-
-inline_for_extraction noextract
-val make_prime_minus_order_k256: unit -> Pure felem4
-  (requires True)
-  (ensures  fun r -> as_nat4 r == S.prime - S.q)
-
-let make_prime_minus_order_k256 () =
-  [@inline_let]
-  let r =
-   (u64 0x402da1722fc9baee,
-    u64 0x4551231950b75fc4,
-    u64 0x1,
-    u64 0x0) in
-
-  assert_norm (as_nat4 r = S.prime - S.q);
-  r
+  BL.is_felem_eq_vartime5_lemma (as_felem5 h0 f1) (as_felem5 h0 f2);
+  BI.is_felem_eq_vartime5
+    (f1.(0ul), f1.(1ul), f1.(2ul), f1.(3ul), f1.(4ul))
+    (f2.(0ul), f2.(1ul), f2.(2ul), f2.(3ul), f2.(4ul))
 
 
 [@CInline]
 let is_felem_lt_prime_minus_order_vartime f =
-  push_frame ();
-  let n = create nlimb (u64 0) in
-  make_u64_4 n (make_prime_minus_order_k256 ());
-
   let h0 = ST.get () in
-  let m = BN.bn_lt_mask nlimb f n in
-  SN.bn_lt_mask_lemma (as_seq h0 f) (as_seq h0 n);
-  pop_frame ();
-  BB.unsafe_bool_of_limb m
-
-
-// needed for Montgomery arithmetic
-inline_for_extraction noextract
-val make_r2_modp: unit -> Pure felem4
-  (requires True)
-  (ensures  fun r -> as_nat4 r = pow2 512 % S.prime)
-
-let make_r2_modp () =
-  assert_norm (pow2 512 % S.prime = 0x1000007a2000e90a1);
-  (u64 0x7a2000e90a1, u64 0x1, u64 0x0, u64 0x0)
-
-
-// needed for Montgomery arithmetic
-inline_for_extraction noextract
-val make_mu0 : unit -> Pure uint64
-  (requires True)
-  (ensures  fun mu -> (1 + S.prime * v mu) % pow2 64 = 0)
-
-let make_mu0 () =
-  assert_norm ((1 + S.prime * 15580212934572586289) % pow2 64 = 0);
-  u64 15580212934572586289
-
-
-val modp: out:felem -> a:lbuffer uint64 (2ul *! nlimb) -> Stack unit
-  (requires fun h ->
-    live h a /\ live h out /\ disjoint a out)
-  (ensures  fun h0 _ h1 -> modifies (loc out) h0 h1 /\
-    as_nat h1 out == BD.bn_v h0 a % S.prime)
-
-[@CInline]
-let modp out a =
-  push_frame ();
-  let n = create nlimb (u64 0) in
-  make_u64_4 n (make_prime_k256 ());
-
-  let r2 = create 4ul (u64 0) in
-  make_u64_4 r2 (make_r2_modp ());
-
-  let mu = make_mu0 () in
-
-  BR.bn_mod_slow_precomp (AM.mk_runtime_almost_mont nlimb) n mu r2 a out;
-  pop_frame ()
+  BL.is_felem_lt_prime_minus_order_vartime5_lemma (as_felem5 h0 f);
+  BI.is_felem_lt_prime_minus_order_vartime5 (f.(0ul), f.(1ul), f.(2ul), f.(3ul), f.(4ul))
 
 
 let create_felem () =
-  SD.bn_eval_zeroes #U64 (v nlimb) (v nlimb);
   create nlimb (u64 0)
 
 
 [@CInline]
 let load_felem f b =
+  push_frame ();
+  let tmp = create 4ul (u64 0) in
   let h0 = ST.get () in
-  SN.bn_from_bytes_be_lemma #U64 32 (as_seq h0 b);
-  BN.bn_from_bytes_be 32ul b f
+  uints_from_bytes_be tmp b;
+  let h1 = ST.get () in
+  assert (as_seq h1 tmp == BSeq.uints_from_bytes_be (as_seq h0 b));
+  BSeq.uints_from_bytes_be_nat_lemma #U64 #_ #4 (as_seq h0 b);
+  assert (BSeq.nat_from_intseq_be (BSeq.uints_from_bytes_be #U64 #_ #4 (as_seq h0 b)) == BSeq.nat_from_bytes_be (as_seq h0 b));
+  BDL.unfold_nat_from_uint64_four (as_seq h1 tmp);
+  assert (BSeq.nat_from_intseq_be (as_seq h1 tmp) == as_nat4 (as_felem4 h1 tmp));
+  BL.load_felem5_lemma (as_felem4 h1 tmp);
+  make_u52_5 f (BI.load_felem5 (tmp.(3ul),tmp.(2ul),tmp.(1ul),tmp.(0ul)));
+  let h2 = ST.get () in
+  assert (as_nat4 (as_felem4 h1 tmp) == as_nat5 (as_felem5 h2 f));
+  pop_frame ()
 
 
 [@CInline]
 let load_felem_vartime f b =
-  push_frame ();
-  let n = create nlimb (u64 0) in
-  make_u64_4 n (make_prime_k256 ());
-
+  load_felem f b;
   let h0 = ST.get () in
-  SN.bn_from_bytes_be_lemma #U64 32 (as_seq h0 b);
-  BN.bn_from_bytes_be 32ul b f;
-  let h1 = ST.get () in
-
-  let is_zero = is_felem_zero_vartime f in
-  let is_lt_p = BN.bn_lt_mask nlimb f n in
-  SN.bn_lt_mask_lemma (as_seq h1 f) (as_seq h0 n);
-  let is_lt_p_b = BB.unsafe_bool_of_limb is_lt_p in
-  pop_frame ();
-  not is_zero && is_lt_p_b
+  let is_ge_p = BI.is_felem_ge_prime_vartime5 (f.(0ul),f.(1ul),f.(2ul),f.(3ul),f.(4ul)) in
+  BL.is_felem_ge_prime_vartime5_lemma (as_felem5 h0 f);
+  if is_ge_p then false
+  else not (is_felem_zero_vartime f)
 
 
 [@CInline]
 let store_felem b f =
+  push_frame ();
+  let tmp = create 4ul (u64 0) in
   let h0 = ST.get () in
-  SN.bn_to_bytes_be_lemma #U64 32 (as_seq h0 f);
-  BN.bn_to_bytes_be 32ul f b
+  make_u64_4 tmp (BI.store_felem5 (f.(0ul),f.(1ul),f.(2ul),f.(3ul),f.(4ul)));
+  let h1 = ST.get () in
+  BL.store_felem5_lemma (as_felem5 h0 f);
+  assert (as_nat4 (as_felem4 h1 tmp) == as_nat5 (as_felem5 h0 f));
+  BDL.unfold_nat_from_uint64_four (as_seq h1 tmp);
+  BSeq.lemma_nat_from_to_intseq_be_preserves_value 4 (as_seq h1 tmp);
+  assert (BSeq.nat_to_intseq_be 4 (BSeq.nat_from_intseq_be (as_seq h1 tmp)) == as_seq h1 tmp);
+  assert (BSeq.nat_to_intseq_be 4 (as_nat5 (as_felem5 h0 f)) == as_seq h1 tmp);
+  uints_to_bytes_be 4ul b tmp;
+  let h2 = ST.get () in
+  assert (as_seq h2 b == BSeq.uints_to_bytes_be (as_seq h1 tmp));
+  assert (as_seq h2 b == BSeq.uints_to_bytes_be #_ #_ #4 (BSeq.nat_to_intseq_be #U64 4 (as_nat5 (as_felem5 h0 f))));
+  BSeq.uints_to_bytes_be_nat_lemma #U64 #SEC 4 (as_nat5 (as_felem5 h0 f));
+  pop_frame ()
 
 
 let set_zero f =
   memset f (u64 0) nlimb;
   let h = ST.get () in
-  assert (as_seq h f == LSeq.create (v nlimb) (u64 0));
-  SD.bn_eval_zeroes #U64 (v nlimb) (v nlimb)
+  assert (as_seq h f == LSeq.create (v nlimb) (u64 0))
 
 
 let set_one f =
-  BN.bn_from_uint nlimb (u64 1) f;
-  SN.bn_from_uint_lemma (v nlimb) (u64 1)
+  set_zero f;
+  f.(0ul) <- u64 1
 
 // not used
 let copy_felem f1 f2 = copy f1 f2
 
+
 [@CInline]
-let fmul_small_num out f1 num =
-  push_frame ();
-  let f2 = create nlimb (u64 0) in
-  BN.bn_from_uint nlimb num f2;
-  SN.bn_from_uint_lemma (v nlimb) num;
-
-  let h0 = ST.get () in
-  let tmp = create (2ul *! nlimb) (u64 0) in
-  BN.bn_mul nlimb nlimb f2 f1 tmp;
-  SN.bn_mul_lemma (as_seq h0 f2) (as_seq h0 f1);
-
-  modp out tmp;
-  pop_frame ()
-
-
-let fmul_3b out f =
-  [@inline_let]
-  let b3 = normalize_term (u64 (S.b * 3)) in
-  fmul_small_num out f b3
-
-
-let fmul_24b out f =
-  [@inline_let]
-  let b24 = normalize_term (u64 (S.b * 24)) in
-  fmul_small_num out f b24
+let fmul_small_num out f num =
+  make_u52_5 out (BI.mul15 (f.(0ul), f.(1ul), f.(2ul), f.(3ul), f.(4ul)) num)
 
 
 [@CInline]
 let fadd out f1 f2 =
-  push_frame ();
-  let n = create nlimb (u64 0) in
-  make_u64_4 n (make_prime_k256 ());
-
-  let h0 = ST.get () in
-  BN.bn_add_mod_n nlimb n f1 f2 out;
-  SN.bn_add_mod_n_lemma (as_seq h0 n) (as_seq h0 f1) (as_seq h0 f2);
-  pop_frame ()
+  make_u52_5 out (BI.add5
+    (f1.(0ul), f1.(1ul), f1.(2ul), f1.(3ul), f1.(4ul))
+    (f2.(0ul), f2.(1ul), f2.(2ul), f2.(3ul), f2.(4ul)))
 
 
 [@CInline]
-let fsub out f1 f2 =
-  push_frame ();
-  let n = create nlimb (u64 0) in
-  make_u64_4 n (make_prime_k256 ());
-
-  let h0 = ST.get () in
-  BN.bn_sub_mod_n nlimb n f1 f2 out;
-  SN.bn_sub_mod_n_lemma (as_seq h0 n) (as_seq h0 f1) (as_seq h0 f2);
-  pop_frame ()
+let fsub out f1 f2 x =
+  make_u52_5 out (BI.fsub5
+    (f1.(0ul), f1.(1ul), f1.(2ul), f1.(3ul), f1.(4ul))
+    (f2.(0ul), f2.(1ul), f2.(2ul), f2.(3ul), f2.(4ul)) x)
 
 
 [@CInline]
 let fmul out f1 f2 =
-  push_frame ();
-  let h0 = ST.get () in
-  let tmp = create (2ul *! nlimb) (u64 0) in
-  BN.bn_mul nlimb nlimb f1 f2 tmp;
-  SN.bn_mul_lemma (as_seq h0 f1) (as_seq h0 f2);
-
-  modp out tmp;
-  pop_frame ()
+  make_u52_5 out (BI.fmul5
+    (f1.(0ul), f1.(1ul), f1.(2ul), f1.(3ul), f1.(4ul))
+    (f2.(0ul), f2.(1ul), f2.(2ul), f2.(3ul), f2.(4ul)))
 
 
 [@CInline]
 let fsqr out f =
-  push_frame ();
-  let h0 = ST.get () in
-  let tmp = create (2ul *! nlimb) (u64 0) in
-  BN.bn_sqr nlimb f tmp;
-  SN.bn_sqr_lemma (as_seq h0 f);
-
-  modp out tmp;
-  pop_frame ()
+  make_u52_5 out (BI.fsqr5 (f.(0ul), f.(1ul), f.(2ul), f.(3ul), f.(4ul)))
