code/k256/Hacl.K256.Field.fsti
@@ -12,80 +12,119 @@ module LSeq = Lib.Sequence
 module BSeq = Lib.ByteSequence
 module S = Spec.K256
 
-module BD = Hacl.Bignum.Definitions
-
+include Hacl.Spec.K256.Field52.Definitions
+module BI = Hacl.Spec.K256.Field52
 
 #set-options "--z3rlimit 50 --fuel 0 --ifuel 0"
 
-(**
-  This is a naive implementation of field arithmetic for testing purposes
-*)
+(** Specialized bignum library with a radix-2^{52} *)
 
 inline_for_extraction noextract
-let nlimb = 4ul
+let nlimb = 5ul
 
 inline_for_extraction noextract
 let felem = lbuffer uint64 nlimb
 
 noextract
-let as_nat (h:mem) (e:felem) : GTot nat = BD.bn_v #U64 #nlimb h e
+let as_felem5 (h:mem) (e:felem) : GTot felem5 =
+  let open Lib.Sequence in
+  let s = as_seq h e in
+  (s.[0], s.[1], s.[2], s.[3], s.[4])
+
+noextract
+let as_nat (h:mem) (e:felem) : GTot nat =
+  as_nat5 (as_felem5 h e)
 
 noextract
 let feval (h:mem) (e:felem) : GTot S.felem = as_nat h e % S.prime
 
 noextract
-let fe_lt_prime (h:mem) (e:felem) = as_nat h e < S.prime
-
-inline_for_extraction noextract
-let felem4 = uint64 & uint64 & uint64 & uint64
+let inv_fully_reduced5 (f:felem5) =
+  felem_fits5 f (1,1,1,1,1) /\
+  as_nat5 f < S.prime
 
 noextract
-let as_nat4 (f:felem4) =
-  let (f0, f1, f2, f3) = f in
-  v f0 + v f1 * pow2 64 + v f2 * pow2 128 + v f3 * pow2 192
+let inv_fully_reduced (h:mem) (e:felem) =
+  let f = as_felem5 h e in
+  inv_fully_reduced5 f
+
+
+noextract
+let inv_lazy_reduced1_5 (f:felem5) =
+  felem_fits5 f (1,1,1,1,1)
+
+noextract
+let inv_lazy_reduced1 (h:mem) (e:felem) =
+  let f = as_felem5 h e in
+  inv_lazy_reduced1_5 f
+
+
+noextract
+let inv_fe_is_fe5 (h:mem) (e:felem) (f:felem5) =
+  let (f0,f1,f2,f3,f4) = f in
+  let (e0,e1,e2,e3,e4) = as_felem5 h e in
+  f0 == e0 /\ f1 == e1 /\ f2 == e2 /\ f3 == e3 /\ f4 == e4
+
+
+noextract
+let as_felem4 (h:mem) (e:lbuffer uint64 4ul) : GTot felem4 =
+  let open Lib.Sequence in
+  let s = as_seq h e in
+  (s.[3], s.[2], s.[1], s.[0])
 
 
 inline_for_extraction noextract
-val make_u64_4 (out:felem) (f:felem4) : Stack unit
+val make_u64_4 (out:lbuffer uint64 4ul) (f:felem4) : Stack unit
   (requires fun h -> live h out)
   (ensures  fun h0 _ h1 -> modifies (loc out) h0 h1 /\
-    as_nat h1 out == as_nat4 f)
+    as_felem4 h1 out == f)
 
 
 inline_for_extraction noextract
-val make_prime_k256: unit -> Pure felem4
-  (requires True)
-  (ensures  fun r -> as_nat4 r = S.prime)
+val make_u52_5 (out:felem) (f:felem5) : Stack unit
+  (requires fun h -> live h out)
+  (ensures  fun h0 _ h1 -> modifies (loc out) h0 h1 /\
+    as_nat h1 out == as_nat5 f /\ inv_fe_is_fe5 h1 out f)
 
 
 inline_for_extraction noextract
-val make_order_k256: unit -> Pure felem4
+val make_prime_k256: unit -> Pure felem5
   (requires True)
-  (ensures  fun r -> as_nat4 r = S.q)
+  (ensures  fun r ->
+    as_nat5 r = S.prime /\ inv_lazy_reduced1_5 r)
 
 
 inline_for_extraction noextract
-val make_b_k256: unit -> Pure felem4
+val make_order_k256: unit -> Pure felem5
   (requires True)
-  (ensures  fun r -> as_nat4 r = S.b)
+  (ensures  fun r ->
+    as_nat5 r = S.q /\ inv_fully_reduced5 r)
+
+
+inline_for_extraction noextract
+val make_b_k256: unit -> Pure felem5
+  (requires True)
+  (ensures  fun r ->
+    as_nat5 r = S.b /\ inv_fully_reduced5 r)
 
 
 val is_felem_zero_vartime (f:felem) : Stack bool
-  (requires fun h -> live h f)
+  (requires fun h -> live h f /\ inv_fully_reduced h f )
   (ensures  fun h0 m h1 -> modifies0 h0 h1 /\
     m == (as_nat h0 f = 0))
 
 
 val is_felem_eq_vartime (f1 f2:felem) : Stack bool
   (requires fun h ->
-    live h f1 /\ live h f2 /\ fe_lt_prime h f1 /\ fe_lt_prime h f2)
+    live h f1 /\ live h f2 /\
+    inv_fully_reduced h f1 /\ inv_fully_reduced h f2)
   (ensures  fun h0 m h1 -> modifies0 h0 h1 /\
     m == (as_nat h0 f1 = as_nat h0 f2))
 
 
 // needed for ecdsa-verify when q < p < 2q
 val is_felem_lt_prime_minus_order_vartime (f:felem) : Stack bool
-  (requires fun h -> live h f /\ fe_lt_prime h f)
+  (requires fun h -> live h f /\ inv_fully_reduced h f)
   (ensures  fun h0 m h1 -> modifies0 h0 h1 /\
     m == (as_nat h0 f < S.prime - S.q))
 
@@ -95,15 +134,16 @@ val create_felem: unit -> StackInline felem
   (requires fun h -> True)
   (ensures  fun h0 f h1 ->
     stack_allocated f h0 h1 (LSeq.create (v nlimb) (u64 0)) /\
-    as_nat h1 f == 0)
+    as_nat h1 f == 0 /\ inv_fully_reduced h1 f)
 
 
+//BSeq.nat_from_bytes_be (as_seq h b) < S.prime
 val load_felem: f:felem -> b:lbuffer uint8 32ul -> Stack unit
   (requires fun h ->
-    live h f /\ live h b /\ disjoint f b /\
-    BSeq.nat_from_bytes_be (as_seq h b) < S.prime)
+    live h f /\ live h b /\ disjoint f b)
   (ensures  fun h0 _ h1 -> modifies (loc f) h0 h1 /\
-    as_nat h1 f == BSeq.nat_from_bytes_be (as_seq h0 b))
+    as_nat h1 f == BSeq.nat_from_bytes_be (as_seq h0 b) /\
+    inv_lazy_reduced1 h1 f)
 
 
 val load_felem_vartime: f:felem -> b:lbuffer uint8 32ul -> Stack bool
@@ -111,13 +151,14 @@ val load_felem_vartime: f:felem -> b:lbuffer uint8 32ul -> Stack bool
     live h f /\ live h b /\ disjoint f b)
   (ensures  fun h0 m h1 -> modifies (loc f) h0 h1 /\
    (let b_nat = BSeq.nat_from_bytes_be (as_seq h0 b) in
-    as_nat h1 f == b_nat /\ m = (0 < b_nat && b_nat < S.prime)))
+    as_nat h1 f == b_nat /\ m = (0 < b_nat && b_nat < S.prime) /\
+    inv_lazy_reduced1 h1 f))
 
 
 val store_felem: b:lbuffer uint8 32ul -> f:felem -> Stack unit
   (requires fun h ->
     live h b /\ live h f /\ disjoint f b /\
-    fe_lt_prime h f)
+    inv_fully_reduced h f)
   (ensures  fun h0 _ h1 -> modifies (loc b) h0 h1 /\
     as_seq h1 b == BSeq.nat_to_bytes_be 32 (as_nat h0 f))
 
@@ -126,14 +167,14 @@ inline_for_extraction noextract
 val set_zero: f:felem -> Stack unit
   (requires fun h -> live h f)
   (ensures  fun h0 _ h1 -> modifies (loc f) h0 h1 /\
-    as_nat h1 f == 0)
+    as_nat h1 f == 0 /\ inv_fully_reduced h1 f)
 
 
 inline_for_extraction noextract
 val set_one: f:felem -> Stack unit
   (requires fun h -> live h f)
   (ensures  fun h0 _ h1 -> modifies (loc f) h0 h1 /\
-    as_nat h1 f == 1)
+    as_nat h1 f == 1 /\ inv_fully_reduced h1 f)
 
 
 // not used
@@ -148,67 +189,37 @@ val copy_felem (f1 f2:felem) : Stack unit
 // num = 3; 2; 8
 val fmul_small_num (out f:felem) (num:uint64) : Stack unit
   (requires fun h -> // v num <= 8 is a maximum value for point addition and doubling
-    live h f /\ live h out /\ eq_or_disjoint out f /\
-    fe_lt_prime h f)
+    live h f /\ live h out /\ eq_or_disjoint out f)
   (ensures  fun h0 _ h1 -> modifies (loc out) h0 h1 /\
-    as_nat h1 out = S.fmul (v num) (as_nat h0 f) /\
-    fe_lt_prime h1 out)
-
-
-inline_for_extraction noextract
-val fmul_3b (out f:felem) : Stack unit
-  (requires fun h ->
-    live h f /\ live h out /\ eq_or_disjoint out f /\
-    fe_lt_prime h f)
-  (ensures  fun h0 _ h1 -> modifies (loc out) h0 h1 /\
-    as_nat h1 out = S.fmul (S.fmul 3 S.b) (as_nat h0 f) /\
-    fe_lt_prime h1 out)
-
-
-inline_for_extraction noextract
-val fmul_24b (out f:felem) : Stack unit
-  (requires fun h ->
-    live h f /\ live h out /\ eq_or_disjoint out f /\
-    fe_lt_prime h f)
-  (ensures  fun h0 _ h1 -> modifies (loc out) h0 h1 /\
-    as_nat h1 out = S.fmul (S.fmul 24 S.b) (as_nat h0 f) /\
-    fe_lt_prime h1 out)
+    inv_fe_is_fe5 h1 out (BI.mul15 (as_felem5 h0 f) num))
 
 
 val fadd (out f1 f2:felem) : Stack unit
   (requires fun h ->
     live h out /\ live h f1 /\ live h f2 /\
-    eq_or_disjoint out f1 /\ eq_or_disjoint out f2 /\ eq_or_disjoint f1 f2 /\
-    fe_lt_prime h f1 /\ fe_lt_prime h f2)
+    eq_or_disjoint out f1 /\ eq_or_disjoint out f2 /\ eq_or_disjoint f1 f2)
   (ensures  fun h0 _ h1 -> modifies (loc out) h0 h1 /\
-    as_nat h1 out == S.fadd (as_nat h0 f1) (as_nat h0 f2) /\
-    fe_lt_prime h1 out)
+    inv_fe_is_fe5 h1 out (BI.add5 (as_felem5 h0 f1) (as_felem5 h0 f2)))
 
 
-val fsub (out f1 f2: felem) : Stack unit
+val fsub (out f1 f2: felem) (x:uint64) : Stack unit
   (requires fun h ->
     live h out /\ live h f1 /\ live h f2 /\
-    eq_or_disjoint out f1 /\ eq_or_disjoint out f2 /\ eq_or_disjoint f1 f2 /\
-    fe_lt_prime h f1 /\ fe_lt_prime h f2)
+    eq_or_disjoint out f1 /\ eq_or_disjoint out f2 /\ eq_or_disjoint f1 f2)
   (ensures  fun h0 _ h1 -> modifies (loc out) h0 h1 /\
-    as_nat h1 out == S.fsub (as_nat h0 f1) (as_nat h0 f2) /\
-    fe_lt_prime h1 out)
+    inv_fe_is_fe5 h1 out (BI.fsub5 (as_felem5 h0 f1) (as_felem5 h0 f2) x))
 
 
 val fmul (out f1 f2: felem) : Stack unit
   (requires fun h ->
     live h out /\ live h f1 /\ live h f2 /\
-    eq_or_disjoint out f1 /\ eq_or_disjoint out f2 /\ eq_or_disjoint f1 f2 /\
-    fe_lt_prime h f1 /\ fe_lt_prime h f2)
+    eq_or_disjoint out f1 /\ eq_or_disjoint out f2 /\ eq_or_disjoint f1 f2)
   (ensures  fun h0 _ h1 -> modifies (loc out) h0 h1 /\
-    as_nat h1 out == S.fmul (as_nat h0 f1) (as_nat h0 f2) /\
-    fe_lt_prime h1 out)
+    inv_fe_is_fe5 h1 out (BI.fmul5 (as_felem5 h0 f1) (as_felem5 h0 f2)))
 
 
 val fsqr (out f: felem) : Stack unit
   (requires fun h ->
-    live h out /\ live h f /\ eq_or_disjoint out f /\
-    fe_lt_prime h f)
+    live h out /\ live h f /\ eq_or_disjoint out f)
   (ensures  fun h0 _ h1 -> modifies (loc out) h0 h1 /\
-    as_nat h1 out == S.fmul (as_nat h0 f) (as_nat h0 f) /\
-    fe_lt_prime h1 out)
+    inv_fe_is_fe5 h1 out (BI.fsqr5 (as_felem5 h0 f)))
